small step

exercises/Smallstep.v
@@ -1,6 +1,81 @@
+(** * Smallstep: Small-step Operational Semantics *)
+
 Require Export Imp.
 
-(* a toy language *)
+
+(** The evaluators we have seen so far (e.g., the ones for
+    [aexp]s, [bexp]s, and commands) have been formulated in a
+    "big-step" style -- they specify how a given expression can be
+    evaluated to its final value (or a command plus a store to a final
+    store) "all in one big step."
+
+    This style is simple and natural for many purposes -- indeed,
+    Gilles Kahn, who popularized its use, called it _natural
+    semantics_.  But there are some things it does not do well.  In
+    particular, it does not give us a natural way of talking about
+    _concurrent_ programming languages, where the "semantics" of a
+    program -- i.e., the essence of how it behaves -- is not just
+    which input states get mapped to which output states, but also
+    includes the intermediate states that it passes through along the
+    way, since these states can also be observed by concurrently
+    executing code.
+
+    Another shortcoming of the big-step style is more technical, but
+    critical in some situations.  To see the issue, suppose we wanted
+    to define a variant of Imp where variables could hold _either_
+    numbers _or_ lists of numbers (see the [HoareList] chapter for
+    details).  In the syntax of this extended language, it will be
+    possible to write strange expressions like [2 + nil], and our
+    semantics for arithmetic expressions will then need to say
+    something about how such expressions behave.  One
+    possibility (explored in the [HoareList] chapter) is to maintain
+    the convention that every arithmetic expressions evaluates to some
+    number by choosing some way of viewing a list as a number -- e.g.,
+    by specifying that a list should be interpreted as [0] when it
+    occurs in a context expecting a number.  But this is really a bit
+    of a hack.
+
+    A much more natural approach is simply to say that the behavior of
+    an expression like [2+nil] is _undefined_ -- it doesn't evaluate
+    to any result at all.  And we can easily do this: we just have to
+    formulate [aeval] and [beval] as [Inductive] propositions rather
+    than Fixpoints, so that we can make them partial functions instead
+    of total ones.
+
+    However, now we encounter a serious deficiency.  In this language,
+    a command might _fail_ to map a given starting state to any ending
+    state for two quite different reasons: either because the
+    execution gets into an infinite loop or because, at some point,
+    the program tries to do an operation that makes no sense, such as
+    adding a number to a list, and none of the evaluation rules can be
+    applied.
+
+    These two outcomes -- nontermination vs. getting stuck in an
+    erroneous configuration -- are quite different.  In particular, we
+    want to allow the first (permitting the possibility of infinite
+    loops is the price we pay for the convenience of programming with
+    general looping constructs like [while]) but prevent the
+    second (which is just wrong), for example by adding some form of
+    _typechecking_ to the language.  Indeed, this will be a major
+    topic for the rest of the course.  As a first step, we need a
+    different way of presenting the semantics that allows us to
+    distinguish nontermination from erroneous "stuck states."
+
+    So, for lots of reasons, we'd like to have a finer-grained way of
+    defining and reasoning about program behaviors.  This is the topic
+    of the present chapter.  We replace the "big-step" [eval] relation
+    with a "small-step" relation that specifies, for a given program,
+    how the "atomic steps" of computation are performed. *)
+
+
+(* ########################################################### *)
+(** * A Toy Language *)
+
+(** To save space in the discussion, let's go back to an
+    incredibly simple language containing just constants and
+    addition.  (We use single letters -- [C] and [P] -- for the
+    constructor names, for brevity.)  At the end of the chapter, we'll
+    see how to apply the same techniques to the full Imp language.  *)
 
 Inductive tm : Type :=
   | C : nat -> tm         (* Constant *)
@@ -10,11 +85,27 @@ Tactic Notation "tm_cases" tactic(first) ident(c) :=
   first;
   [ Case_aux c "C" | Case_aux c "P" ].
 
+(** Here is a standard evaluator for this language, written in the
+    same (big-step) style as we've been using up to this point. *)
+
 Fixpoint evalF (t : tm) : nat :=
   match t with
   | C n => n
   | P a1 a2 => evalF a1 + evalF a2
   end.
+
+(** Now, here is the same evaluator, written in exactly the same
+    style, but formulated as an inductively defined relation.  Again,
+    we use the notation [t || n] for "[t] evaluates to [n]." *)
+(**
+                               --------                                (E_Const)
+                               C n || n
+
+                               t1 || n1
+                               t2 || n2
+                        ----------------------                         (E_Plus)
+                        P t1 t2 || C (n1 + n2)
+*)
 
 Reserved Notation " t '||' n " (at level 50, left associativity).
 
@@ -33,6 +124,22 @@ Tactic Notation "eval_cases" tactic(first) ident(c) :=
   [ Case_aux c "E_Const" | Case_aux c "E_Plus" ].
 
 Module SimpleArith1.
+
+(** Now, here is a small-step version. *)
+(**
+                     -------------------------------        (ST_PlusConstConst)
+                     P (C n1) (C n2) ==> C (n1 + n2)
+
+                              t1 ==> t1'
+                         --------------------                        (ST_Plus1)
+                         P t1 t2 ==> P t1' t2
+
+                              t2 ==> t2'
+                      ---------------------------                    (ST_Plus2)
+                      P (C n1) t2 ==> P (C n1) t2'
+*)
+
+
 
 Reserved Notation " t '==>' t' " (at level 40).
 
@@ -53,6 +160,25 @@ Tactic Notation "step_cases" tactic(first) ident(c) :=
   [ Case_aux c "ST_PlusConstConst"
   | Case_aux c "ST_Plus1" | Case_aux c "ST_Plus2" ].
 
+(** Things to notice:
+
+    - We are defining just a single reduction step, in which
+      one [P] node is replaced by its value.
+
+    - Each step finds the _leftmost_ [P] node that is ready to
+      go (both of its operands are constants) and rewrites it in
+      place.  The first rule tells how to rewrite this [P] node
+      itself; the other two rules tell how to find it.
+
+    - A term that is just a constant cannot take a step. *)
+
+
+(** Let's pause and check a couple of examples of reasoning with
+    the [step] relation... *)
+
+(** If [t1] can take a step to [t1'], then [P t1 t2] steps
+    to [P t1' t2]: *)
+
 Example test_step_1 :
       P
         (P (C 0) (C 3))
@@ -64,7 +190,11 @@ Example test_step_1 :
 Proof.
   apply ST_Plus1. apply ST_PlusConstConst.  Qed.
 
-(* Exercise: 1 star (test_step_2) *)
+(** **** Exercise: 1 star (test_step_2)  *)
+(** Right-hand sides of sums can take a step only when the
+    left-hand side is finished: if [t2] can take a step to [t2'],
+    then [P (C n) t2] steps to [P (C n)
+    t2']: *)
 
 Example test_step_2 :
       P
@@ -82,10 +212,64 @@ Proof.
   repeat (apply ST_Plus2).
   apply ST_PlusConstConst.
 Qed.
+(** [] *)
 
-(* Relations *)
+
+
+
+(* ########################################################### *)
+(** * Relations *)
+
+(** We will be using several different step relations, so it is
+    helpful to generalize a bit and state a few definitions and
+    theorems about relations in general.  (The optional chapter
+    [Rel.v] develops some of these ideas in a bit more detail; it may
+    be useful if the treatment here is too dense.) *)
+
+(** A (binary) _relation_ on a set [X] is a family of propositions
+    parameterized by two elements of [X] -- i.e., a proposition about
+    pairs of elements of [X].  *)
 
 Definition relation (X: Type) := X->X->Prop.
+
+
+(** Our main examples of such relations in this chapter will be
+    the single-step and multi-step reduction relations on terms, [==>]
+    and [==>*], but there are many other examples -- some that come to
+    mind are the "equals," "less than," "less than or equal to," and
+    "is the square of" relations on numbers, and the "prefix of"
+    relation on lists and strings. *)
+
+
+(** One simple property of the [==>] relation is that, like the
+    evaluation relation for our language of Imp programs, it is
+    _deterministic_.
+
+    _Theorem_: For each [t], there is at most one [t'] such that [t]
+    steps to [t'] ([t ==> t'] is provable).  Formally, this is the
+    same as saying that [==>] is deterministic. *)
+
+(** _Proof sketch_: We show that if [x] steps to both [y1] and [y2]
+    then [y1] and [y2] are equal, by induction on a derivation of
+    [step x y1].  There are several cases to consider, depending on
+    the last rule used in this derivation and in the given derivation
+    of [step x y2].
+
+      - If both are [ST_PlusConstConst], the result is immediate.
+
+      - The cases when both derivations end with [ST_Plus1] or
+        [ST_Plus2] follow by the induction hypothesis.
+
+      - It cannot happen that one is [ST_PlusConstConst] and the other
+        is [ST_Plus1] or [ST_Plus2], since this would imply that [x] has
+        the form [P t1 t2] where both [t1] and [t2] are
+        constants (by [ST_PlusConstConst]) _and_ one of [t1] or [t2] has
+        the form [P ...].
+
+      - Similarly, it cannot happen that one is [ST_Plus1] and the other
+        is [ST_Plus2], since this would imply that [x] has the form
+        [P t1 t2] where [t1] has both the form [P t1 t2] and
+        the form [C n]. [] *)
 
 Definition deterministic {X: Type} (R: relation X) :=
   forall x y1 y2 : X, R x y1 -> R x y2 -> y1 = y2.
@@ -114,6 +298,23 @@ Proof.
         reflexivity. assumption.
 Qed.
 
+(** There is some annoying repetition in this proof.
+    Each use of [inversion Hy2] results in three subcases,
+    only one of which is relevant (the one which matches the
+    current case in the induction on [Hy1]). The other two
+    subcases need to be dismissed by finding the contradiction
+    among the hypotheses and doing inversion on it.
+
+    There is a tactic called [solve by inversion] defined in [SfLib.v]
+    that can be of use in such cases. It will solve the goal if it
+    can be solved by inverting some hypothesis; otherwise, it fails.
+    (There are variants [solve by inversion 2] and [solve by inversion 3]
+    that work if two or three consecutive inversions will solve the goal.)
+
+    The example below shows how a proof of the previous theorem can be
+    simplified using this tactic.
+*)
+
 Theorem step_deterministic_alt: deterministic step.
 Proof.
   intros x y1 y2 Hy1 Hy2.
@@ -130,8 +331,68 @@ Qed.
 
 End SimpleArith1.
 
+(* ########################################################### *)
+(** ** Values *)
+
+(** Let's take a moment to slightly generalize the way we state the
+    definition of single-step reduction.  *)
+
+(** It is useful to think of the [==>] relation as defining an
+    _abstract machine_:
+
+      - At any moment, the _state_ of the machine is a term.
+
+      - A _step_ of the machine is an atomic unit of computation --
+        here, a single "add" operation.
+
+      - The _halting states_ of the machine are ones where there is no
+        more computation to be done.
+*)
+(**
+    We can then execute a term [t] as follows:
+
+      - Take [t] as the starting state of the machine.
+
+      - Repeatedly use the [==>] relation to find a sequence of
+        machine states, starting with [t], where each state steps to
+        the next.
+
+      - When no more reduction is possible, "read out" the final state
+        of the machine as the result of execution. *)
+
+(** Intuitively, it is clear that the final states of the
+    machine are always terms of the form [C n] for some [n].
+    We call such terms _values_. *)
+
 Inductive value : tm -> Prop :=
   v_const : forall n, value (C n).
+
+(** Having introduced the idea of values, we can use it in the
+    definition of the [==>] relation to write [ST_Plus2] rule in a
+    slightly more elegant way: *)
+
+(**
+                     -------------------------------        (ST_PlusConstConst)
+                     P (C n1) (C n2) ==> C (n1 + n2)
+
+                              t1 ==> t1'
+                         --------------------                        (ST_Plus1)
+                         P t1 t2 ==> P t1' t2
+
+                               value v1
+                              t2 ==> t2'
+                         --------------------                        (ST_Plus2)
+                         P v1 t2 ==> P v1 t2'
+*)
+(** Again, the variable names here carry important information:
+    by convention, [v1] ranges only over values, while [t1] and [t2]
+    range over arbitrary terms.  (Given this convention, the explicit
+    [value] hypothesis is arguably redundant.  We'll keep it for now,
+    to maintain a close correspondence between the informal and Coq
+    versions of the rules, but later on we'll drop it in informal
+    rules, for the sake of brevity.) *)
+
+(**  Here are the formal rules: *)
 
 Reserved Notation " t '==>' t' " (at level 40).
 
@@ -154,7 +415,32 @@ Tactic Notation "step_cases" tactic(first) ident(c) :=
   [ Case_aux c "ST_PlusConstConst"
   | Case_aux c "ST_Plus1" | Case_aux c "ST_Plus2" ].
 
-(* Exercise: 3 stars (redo_determinism) *)
+(** **** Exercise: 3 stars (redo_determinism)  *)
+(** As a sanity check on this change, let's re-verify determinism
+
+    Proof sketch: We must show that if [x] steps to both [y1] and [y2]
+    then [y1] and [y2] are equal.  Consider the final rules used in
+    the derivations of [step x y1] and [step x y2].
+
+    - If both are [ST_PlusConstConst], the result is immediate.
+
+    - It cannot happen that one is [ST_PlusConstConst] and the other
+      is [ST_Plus1] or [ST_Plus2], since this would imply that [x] has
+      the form [P t1 t2] where both [t1] and [t2] are
+      constants (by [ST_PlusConstConst]) AND one of [t1] or [t2] has
+      the form [P ...].
+
+    - Similarly, it cannot happen that one is [ST_Plus1] and the other
+      is [ST_Plus2], since this would imply that [x] has the form
+      [P t1 t2] where [t1] both has the form [P t1 t2] and
+      is a value (hence has the form [C n]).
+
+    - The cases when both derivations end with [ST_Plus1] or
+      [ST_Plus2] follow by the induction hypothesis. [] *)
+
+(** Most of this proof is the same as the one above.  But to get
+    maximum benefit from the exercise you should try to write it from
+    scratch and just use the earlier one if you get stuck. *)
 
 Theorem step_deterministic :
   deterministic step.
@@ -171,8 +457,37 @@ Proof.
     inversion H. subst. inversion H5.
     rewrite (IHstep t2'0). reflexivity. assumption.
 Qed.
+(** [] *)
 
-(* Strong Progress and Normal Forms *)
+(* ########################################################### *)
+(** ** Strong Progress and Normal Forms *)
+
+(** The definition of single-step reduction for our toy language is
+    fairly simple, but for a larger language it would be pretty easy
+    to forget one of the rules and create a situation where some term
+    cannot take a step even though it has not been completely reduced
+    to a value.  The following theorem shows that we did not, in fact,
+    make such a mistake here. *)
+
+(** _Theorem_ (_Strong Progress_): If [t] is a term, then either [t]
+    is a value, or there exists a term [t'] such that [t ==> t']. *)
+
+(** _Proof_: By induction on [t].
+
+    - Suppose [t = C n]. Then [t] is a [value].
+
+    - Suppose [t = P t1 t2], where (by the IH) [t1] is either a
+      value or can step to some [t1'], and where [t2] is either a
+      value or can step to some [t2']. We must show [P t1 t2] is
+      either a value or steps to some [t'].
+
+      - If [t1] and [t2] are both values, then [t] can take a step, by
+        [ST_PlusConstConst].
+
+      - If [t1] is a value and [t2] can take a step, then so can [t],
+        by [ST_Plus2].
+
+      - If [t1] can take a step, then so can [t], by [ST_Plus1].  [] *)
 
 Theorem strong_progress : forall t,
   value t \/ (exists t', t ==> t').
@@ -191,8 +506,33 @@ Proof.
           exists (P t' t2).
           apply ST_Plus1. apply H0.  Qed.
 
+(** This important property is called _strong progress_, because
+    every term either is a value or can "make progress" by stepping to
+    some other term.  (The qualifier "strong" distinguishes it from a
+    more refined version that we'll see in later chapters, called
+    simply "progress.") *)
+
+(** The idea of "making progress" can be extended to tell us something
+    interesting about [value]s: in this language [value]s are exactly
+    the terms that _cannot_ make progress in this sense.
+
+    To state this observation formally, let's begin by giving a name
+    to terms that cannot make progress.  We'll call them _normal
+    forms_. *)
+
 Definition normal_form {X:Type} (R:relation X) (t:X) : Prop :=
   ~ exists t', R t t'.
+
+(** This definition actually specifies what it is to be a normal form
+    for an _arbitrary_ relation [R] over an arbitrary set [X], not
+    just for the particular single-step reduction relation over terms
+    that we are interested in at the moment.  We'll re-use the same
+    terminology for talking about other relations later in the
+    course. *)
+
+(** We can use this terminology to generalize the observation we made
+    in the strong progress theorem: in this language, normal forms and
+    values are actually the same thing. *)
 
 Lemma value_is_nf : forall v,
   value v -> normal_form step v.
@@ -216,7 +556,23 @@ Corollary nf_same_as_value : forall t,
 Proof.
   split. apply nf_is_value. apply value_is_nf. Qed.
 
+(** Why is this interesting?
+
+    Because [value] is a syntactic concept -- it is defined by looking
+    at the form of a term -- while [normal_form] is a semantic one --
+    it is defined by looking at how the term steps.  It is not obvious
+    that these concepts should coincide!
+
+    Indeed, we could easily have written the definitions so that they
+    would not coincide... *)
+
+(* ##################################################### *)
+
+(** We might, for example, mistakenly define [value] so that it
+    includes some terms that are not finished reducing. *)
+
 Module Temp1.
+(* Open an inner module so we can redefine value and step. *)
 
 Inductive value : tm -> Prop :=
 | v_const : forall n, value (C n)
@@ -238,8 +594,9 @@ Inductive step : tm -> tm -> Prop :=
 
   where " t '==>' t' " := (step t t').
 
-(* Exercise: 3 stars, advanced (value_not_same_as_normal_form) *)
 
+
+(** **** Exercise: 3 stars, advanced (value_not_same_as_normal_form)  *)
 Lemma value_not_same_as_normal_form :
   exists v, value v /\ ~ normal_form step v.
 Proof.
@@ -247,8 +604,12 @@ Proof.
   constructor.
   unfold normal_form. unfold not. intros. apply H. exists (C (1 + 2)). constructor.
 Qed.
-
+(** [] *)
 End Temp1.
+
+(* ##################################################### *)
+(** Alternatively, we might mistakenly define [step] so that it
+    permits something designated as a value to reduce further. *)
 
 Module Temp2.
 
@@ -272,8 +633,8 @@ Inductive step : tm -> tm -> Prop :=
 
   where " t '==>' t' " := (step t t').
 
-(* Exercise: 2 stars, advanced (value_not_same_as_normal_form) *)
 
+(** **** Exercise: 2 stars, advanced (value_not_same_as_normal_form)  *)
 Lemma value_not_same_as_normal_form :
   exists v, value v /\ ~ normal_form step v.
 Proof.
@@ -281,8 +642,16 @@ Proof.
   split. constructor.
   unfold normal_form. unfold not. intros. apply H. exists (P (C 1) (C 0)). constructor.
 Qed.
-
+(** [] *)
 End Temp2.
+
+(* ########################################################### *)
+(** Finally, we might define [value] and [step] so that there is some
+    term that is not a value but that cannot take a step in the [step]
+    relation.  Such terms are said to be _stuck_. In this case this is
+    caused by a mistake in the semantics, but we will also see
+    situations where, even in a correct language definition, it makes
+    sense to allow some terms to be stuck. *)
 
 Module Temp3.
 
@@ -300,8 +669,9 @@ Inductive step : tm -> tm -> Prop :=
 
   where " t '==>' t' " := (step t t').
 
-(** **** Exercise: 3 stars, advanced (value_not_same_as_normal_form')  *)
+(** (Note that [ST_Plus2] is missing.) *)
 
+(** **** Exercise: 3 stars, advanced (value_not_same_as_normal_form')  *)
 Lemma value_not_same_as_normal_form :
   exists t, ~ value t /\ normal_form step t.
 Proof.
@@ -309,12 +679,18 @@ Proof.
   split. unfold not. intros. inversion H.
   unfold normal_form. unfold not. intros. solve by inversion 3.
 Qed.
+(** [] *)
 
 End Temp3.
 
-(* Additional Exercises *)
+(* ########################################################### *)
+(** *** Additional Exercises *)
 
 Module Temp4.
+
+(** Here is another very simple language whose terms, instead of being
+    just plus and numbers, are just the booleans true and false and a
+    conditional expression... *)
 
 Inductive tm : Type :=
   | ttrue : tm
@@ -338,32 +714,77 @@ Inductive step : tm -> tm -> Prop :=
 
   where " t '==>' t' " := (step t t').
 
-(* Exercise: 3 stars, optional (progress_bool) *)
+(** **** Exercise: 1 star (smallstep_bools)  *)
+(** Which of the following propositions are provable?  (This is just a
+    thought exercise, but for an extra challenge feel free to prove
+    your answers in Coq.) *)
+
+Definition bool_step_prop1 :=
+  tfalse ==> tfalse.
+
+(* FILL IN HERE *)
+
+Definition bool_step_prop2 :=
+     tif
+       ttrue
+       (tif ttrue ttrue ttrue)
+       (tif tfalse tfalse tfalse)
+  ==>
+     ttrue.
+
+(* FILL IN HERE *)
+
+Definition bool_step_prop3 :=
+     tif
+       (tif ttrue ttrue ttrue)
+       (tif ttrue ttrue ttrue)
+       tfalse
+   ==>
+     tif
+       ttrue
+       (tif ttrue ttrue ttrue)
+       tfalse.
+
+(* FILL IN HERE *)
+(** [] *)
+
+(** **** Exercise: 3 stars, optional (progress_bool)  *)
+(** Just as we proved a progress theorem for plus expressions, we can
+    do so for boolean expressions, as well. *)
 
 Theorem strong_progress : forall t,
   value t \/ (exists t', t ==> t').
 Proof.
-  intros.
-  induction t; try(left; constructor).
-  right. inversion IHt1.
-  inversion H. exists t2. constructor. exists t3. constructor.
-  inversion H. exists (tif x t2 t3). constructor. apply H0.
-Qed.
+  (* FILL IN HERE *) Admitted.
+(** [] *)
 
-(* Exercise: 2 stars, optional (step_deterministic) *)
-
+(** **** Exercise: 2 stars, optional (step_deterministic)  *)
 Theorem step_deterministic :
   deterministic step.
 Proof.
-  unfold deterministic. intros.
-  generalize dependent y2.
-  induction H; intros; inversion H0; subst; try(reflexivity); try(solve by inversion).
-  rewrite (IHstep t1'0). reflexivity. apply H5.
-Qed.
+  (* FILL IN HERE *) Admitted.
+(** [] *)
 
 Module Temp5.
 
-(* Exercise: 2 stars (smallstep_bool_shortcut) *)
+(** **** Exercise: 2 stars (smallstep_bool_shortcut)  *)
+(** Suppose we want to add a "short circuit" to the step relation for
+    boolean expressions, so that it can recognize when the [then] and
+    [else] branches of a conditional are the same value (either
+    [ttrue] or [tfalse]) and reduce the whole conditional to this
+    value in a single step, even if the guard has not yet been reduced
+    to a value. For example, we would like this proposition to be
+    provable:
+         tif
+            (tif ttrue ttrue ttrue)
+            tfalse
+            tfalse
+     ==>
+         tfalse.
+*)
+
+(** Write an extra clause for the step relation that achieves this
+    effect and prove [bool_step_prop4]. *)
 
 Reserved Notation " t '==>' t' " (at level 40).
 
@@ -375,8 +796,7 @@ Inductive step : tm -> tm -> Prop :=
   | ST_If : forall t1 t1' t2 t3,
       t1 ==> t1' ->
       tif t1 t2 t3 ==> tif t1' t2 t3
-  | ST_ShortCircuit : forall t1 t2,
-      tif t1 t2 t2 ==> t2
+(* FILL IN HERE *)
 
   where " t '==>' t' " := (step t t').
 
@@ -391,14 +811,69 @@ Definition bool_step_prop4 :=
 Example bool_step_prop4_holds :
   bool_step_prop4.
 Proof.
-  unfold bool_step_prop4.
-  constructor.
-Qed.
+  (* FILL IN HERE *) Admitted.
+(** [] *)
+
+(** **** Exercise: 3 stars, optional (properties_of_altered_step)  *)
+(** It can be shown that the determinism and strong progress theorems
+    for the step relation in the lecture notes also hold for the
+    definition of step given above.  After we add the clause
+    [ST_ShortCircuit]...
+
+    - Is the [step] relation still deterministic?  Write yes or no and
+      briefly (1 sentence) explain your answer.
+
+      Optional: prove your answer correct in Coq.
+*)
+
+(* FILL IN HERE *)
+(**
+   - Does a strong progress theorem hold? Write yes or no and
+     briefly (1 sentence) explain your answer.
+
+     Optional: prove your answer correct in Coq.
+*)
+
+(* FILL IN HERE *)
+(**
+   - In general, is there any way we could cause strong progress to
+     fail if we took away one or more constructors from the original
+     step relation? Write yes or no and briefly (1 sentence) explain
+     your answer.
+
+(* FILL IN HERE *)
+*)
+(** [] *)
 
 End Temp5.
 End Temp4.
 
-(* Multi-Step Reduction *)
+(* ########################################################### *)
+(** * Multi-Step Reduction *)
+
+(** Until now, we've been working with the _single-step reduction_
+    relation [==>], which formalizes the individual steps of an
+    _abstract machine_ for executing programs.
+
+    We can also use this machine to reduce programs to completion --
+    to find out what final result they yield.  This can be formalized
+    as follows:
+
+    - First, we define a _multi-step reduction relation_ [==>*], which
+      relates terms [t] and [t'] if [t] can reach [t'] by any number
+      of single reduction steps (including zero steps!).
+
+    - Then we define a "result" of a term [t] as a normal form that
+      [t] can reach by multi-step reduction. *)
+
+(* ########################################################### *)
+
+(** Since we'll want to reuse the idea of multi-step reduction many
+    times in this and future chapters, let's take a little extra
+    trouble here and define it generically.
+
+    Given a relation [R], we define a relation [multi R], called the
+    _multi-step closure of [R]_ as follows: *)
 
 Inductive multi {X:Type} (R: relation X) : relation X :=
   | multi_refl  : forall (x : X), multi R x x
@@ -407,17 +882,51 @@ Inductive multi {X:Type} (R: relation X) : relation X :=
                     multi R y z ->
                     multi R x z.
 
+(** The effect of this definition is that [multi R] relates two
+    elements [x] and [y] if either
+
+       - [x = y], or else
+       - there is some sequence [z1], [z2], ..., [zn]
+         such that
+           R x z1
+           R z1 z2
+           ...
+           R zn y.
+
+    Thus, if [R] describes a single-step of computation, [z1],
+    ... [zn] is the sequence of intermediate steps of computation
+    between [x] and [y].
+*)
+
 Tactic Notation "multi_cases" tactic(first) ident(c) :=
   first;
   [ Case_aux c "multi_refl" | Case_aux c "multi_step" ].
 
+(** We write [==>*] for the [multi step] relation -- i.e., the
+    relation that relates two terms [t] and [t'] if we can get from
+    [t] to [t'] using the [step] relation zero or more times. *)
+
 Notation " t '==>*' t' " := (multi step t t') (at level 40).
+
+(** The relation [multi R] has several crucial properties.
+
+    First, it is obviously _reflexive_ (that is, [forall x, multi R x
+    x]).  In the case of the [==>*] (i.e. [multi step]) relation, the
+    intuition is that a term can execute to itself by taking zero
+    steps of execution.
+
+    Second, it contains [R] -- that is, single-step executions are a
+    particular case of multi-step executions.  (It is this fact that
+    justifies the word "closure" in the term "multi-step closure of
+    [R].") *)
 
 Theorem multi_R : forall (X:Type) (R:relation X) (x y : X),
        R x y -> (multi R) x y.
 Proof.
   intros X R x y H.
   apply multi_step with y. apply H. apply multi_refl.   Qed.
+
+(** Third, [multi R] is _transitive_. *)
 
 Theorem multi_trans :
   forall (X:Type) (R: relation X) (x y z : X),
@@ -432,7 +941,10 @@ Proof.
       apply multi_step with y. assumption.
       apply IHG. assumption.  Qed.
 
-(* Examples *)
+(** That is, if [t1==>*t2] and [t2==>*t3], then [t1==>*t3]. *)
+
+(* ########################################################### *)
+(** ** Examples *)
 
 Lemma test_multistep_1:
       P
@@ -455,11 +967,28 @@ Proof.
   apply multi_R.
   apply ST_PlusConstConst. Qed.
 
+(** Here's an alternate proof that uses [eapply] to avoid explicitly
+    constructing all the intermediate terms. *)
+
+Lemma test_multistep_1':
+      P
+        (P (C 0) (C 3))
+        (P (C 2) (C 4))
+  ==>*
+      C ((0 + 3) + (2 + 4)).
+Proof.
+  eapply multi_step. apply ST_Plus1. apply ST_PlusConstConst.
+  eapply multi_step. apply ST_Plus2. apply v_const.
+  apply ST_PlusConstConst.
+  eapply multi_step. apply ST_PlusConstConst.
+  apply multi_refl.  Qed.
+
 (** **** Exercise: 1 star, optional (test_multistep_2)  *)
 Lemma test_multistep_2:
   C 3 ==>* C 3.
 Proof.
-  constructor. Qed.
+  (* FILL IN HERE *) Admitted.
+(** [] *)
 
 (** **** Exercise: 1 star, optional (test_multistep_3)  *)
 Lemma test_multistep_3:
@@ -467,7 +996,8 @@ Lemma test_multistep_3:
    ==>*
       P (C 0) (C 3).
 Proof.
-  constructor. Qed.
+  (* FILL IN HERE *) Admitted.
+(** [] *)
 
 (** **** Exercise: 2 stars (test_multistep_4)  *)
 Lemma test_multistep_4:
@@ -481,20 +1011,26 @@ Lemma test_multistep_4:
         (C 0)
         (C (2 + (0 + 3))).
 Proof.
-  apply multi_step with (P (C 0) (P (C 2) (C (0 + 3)))).
-  repeat (apply ST_Plus2). constructor. constructor.
-  apply ST_PlusConstConst.
-  apply multi_step with (P (C 0) (C (2 + (0 + 3)))).
-  apply ST_Plus2. constructor. apply ST_PlusConstConst.
-  constructor.
-Qed.
+  (* FILL IN HERE *) Admitted.
+(** [] *)
 
-(* Normal Forms Again *)
+(* ########################################################### *)
+(** ** Normal Forms Again *)
+
+(** If [t] reduces to [t'] in zero or more steps and [t'] is a
+    normal form, we say that "[t'] is a normal form of [t]." *)
 
 Definition step_normal_form := normal_form step.
 
 Definition normal_form_of (t t' : tm) :=
   (t ==>* t' /\ step_normal_form t').
+
+(** We have already seen that, for our language, single-step reduction is
+    deterministic -- i.e., a given term can take a single step in
+    at most one way.  It follows from this that, if [t] can reach
+    a normal form, then this normal form is unique.  In other words, we
+    can actually pronounce [normal_form t t'] as "[t'] is _the_
+    normal form of [t]." *)
 
 (** **** Exercise: 3 stars, optional (normal_forms_unique)  *)
 Theorem normal_forms_unique:
@@ -503,22 +1039,27 @@ Proof.
   unfold deterministic. unfold normal_form_of.  intros x y1 y2 P1 P2.
   inversion P1 as [P11 P12]; clear P1. inversion P2 as [P21 P22]; clear P2.
   generalize dependent y2.
-  multi_cases (induction P11) Case; intros.
-  Case "multi_refl".
-    multi_cases (inversion P21) SCase.
-    reflexivity.
-    apply ex_falso_quodlibet. apply P12. exists y. assumption.
-  Case "multi_step".
-    multi_cases (inversion P21) SCase; subst.
-    apply ex_falso_quodlibet. apply P22. exists y. apply H.
-    apply IHP11. apply P12.
-      assert (y0 = y). apply (step_deterministic x y0 y); assumption.
-      subst. assumption. assumption.
-Qed.
+  (* We recommend using this initial setup as-is! *)
+  (* FILL IN HERE *) Admitted.
+(** [] *)
+
+(** Indeed, something stronger is true for this language (though not
+    for all languages): the reduction of _any_ term [t] will
+    eventually reach a normal form -- i.e., [normal_form_of] is a
+    _total_ function.  Formally, we say the [step] relation is
+    _normalizing_. *)
 
 Definition normalizing {X:Type} (R:relation X) :=
   forall t, exists t',
     (multi R) t t' /\ normal_form R t'.
+
+(** To prove that [step] is normalizing, we need a couple of lemmas.
+
+    First, we observe that, if [t] reduces to [t'] in many steps, then
+    the same sequence of reduction steps within [t] is also possible
+    when [t] appears as the left-hand child of a [P] node, and
+    similarly when [t] appears as the right-hand child of a [P]
+    node whose left-hand child is a value. *)
 
 Lemma multistep_congr_1 : forall t1 t1' t2,
      t1 ==>* t1' ->
@@ -536,12 +1077,31 @@ Lemma multistep_congr_2 : forall t1 t2 t2',
      t2 ==>* t2' ->
      P t1 t2 ==>* P t1 t2'.
 Proof.
-  intros. multi_cases (induction H0) Case.
-  Case "multi_refl". constructor.
-  Case "multi_step". apply multi_step with (P t1 y).
-    apply ST_Plus2; assumption.
-    assumption.
-Qed.
+  (* FILL IN HERE *) Admitted.
+(** [] *)
+
+(** _Theorem_: The [step] function is normalizing -- i.e., for every
+    [t] there exists some [t'] such that [t] steps to [t'] and [t'] is
+    a normal form.
+
+    _Proof sketch_: By induction on terms.  There are two cases to
+    consider:
+
+    - [t = C n] for some [n].  Here [t] doesn't take a step,
+      and we have [t' = t].  We can derive the left-hand side by
+      reflexivity and the right-hand side by observing (a) that values
+      are normal forms (by [nf_same_as_value]) and (b) that [t] is a
+      value (by [v_const]).
+
+    - [t = P t1 t2] for some [t1] and [t2].  By the IH, [t1] and
+      [t2] have normal forms [t1'] and [t2'].  Recall that normal
+      forms are values (by [nf_same_as_value]); we know that [t1' =
+      C n1] and [t2' = C n2], for some [n1] and [n2].
+      We can combine the [==>*] derivations for [t1] and [t2] to prove
+      that [P t1 t2] reduces in many steps to [C (n1 + n2)].
+
+      It is clear that our choice of [t' = C (n1 + n2)] is a
+      value, which is in turn a normal form. [] *)
 
 Theorem step_normalizing :
   normalizing step.
@@ -575,23 +1135,59 @@ Proof.
         SCase "r".
           rewrite nf_same_as_value. apply v_const.  Qed.
 
-(* Equivalence of Big-Step and Small-Step Reduction *)
+(* ########################################################### *)
+(** ** Equivalence of Big-Step and Small-Step Reduction *)
+
+(** Having defined the operational semantics of our tiny programming
+    language in two different styles, it makes sense to ask whether
+    these definitions actually define the same thing!  They do, though
+    it takes a little work to show it.  (The details are left as an
+    exercise). *)
 
 (** **** Exercise: 3 stars (eval__multistep)  *)
-
 Theorem eval__multistep : forall t n,
   t || n -> t ==>* C n.
+
+(** The key idea behind the proof comes from the following picture:
+       P t1 t2 ==>            (by ST_Plus1)
+       P t1' t2 ==>           (by ST_Plus1)
+       P t1'' t2 ==>          (by ST_Plus1)
+       ...
+       P (C n1) t2 ==>        (by ST_Plus2)
+       P (C n1) t2' ==>       (by ST_Plus2)
+       P (C n1) t2'' ==>      (by ST_Plus2)
+       ...
+       P (C n1) (C n2) ==>    (by ST_PlusConstConst)
+       C (n1 + n2)
+    That is, the multistep reduction of a term of the form [P t1 t2]
+    proceeds in three phases:
+       - First, we use [ST_Plus1] some number of times to reduce [t1]
+         to a normal form, which must (by [nf_same_as_value]) be a
+         term of the form [C n1] for some [n1].
+       - Next, we use [ST_Plus2] some number of times to reduce [t2]
+         to a normal form, which must again be a term of the form [C
+         n2] for some [n2].
+       - Finally, we use [ST_PlusConstConst] one time to reduce [P (C
+         n1) (C n2)] to [C (n1 + n2)]. *)
+
+(** To formalize this intuition, you'll need to use the congruence
+    lemmas from above (you might want to review them now, so that
+    you'll be able to recognize when they are useful), plus some basic
+    properties of [==>*]: that it is reflexive, transitive, and
+    includes [==>]. *)
+
 Proof.
-  intros.
-  eval_cases (induction H) Case.
-  Case "E_Const". constructor.
-  Case "E_Plus". apply multi_trans with (P (C n1) (C n2)).
-    apply multi_trans with (P (C n1) t2).
-    apply multistep_congr_1. assumption.
-    apply multistep_congr_2. apply nf_same_as_value. apply value_is_nf. constructor. assumption.
-    apply multi_step with (C (n1 + n2)).
-    apply ST_PlusConstConst. constructor.
-Qed.
+  (* FILL IN HERE *) Admitted.
+(** [] *)
+
+(** **** Exercise: 3 stars, advanced (eval__multistep_inf)  *)
+(** Write a detailed informal version of the proof of [eval__multistep].
+
+(* FILL IN HERE *)
+[]
+*)
+(** For the other direction, we need one lemma, which establishes a
+    relation between single-step reduction and big-step evaluation. *)
 
 (** **** Exercise: 3 stars (step__eval)  *)
 Lemma step__eval : forall t t' n,
@@ -600,49 +1196,45 @@ Lemma step__eval : forall t t' n,
      t || n.
 Proof.
   intros t t' n Hs. generalize dependent n.
-  step_cases (induction Hs) Case; intros.
-  Case "ST_PlusConstConst".
-    inversion H. apply E_Plus; constructor.
-  Case "ST_Plus1".
-    inversion H. apply E_Plus. apply IHHs. assumption. assumption.
-  Case "ST_Plus2".
-    inversion H0. apply E_Plus. assumption. apply IHHs. assumption.
-Qed.
+  (* FILL IN HERE *) Admitted.
+(** [] *)
 
+(** The fact that small-step reduction implies big-step is now
+    straightforward to prove, once it is stated correctly.
 
-(* Exercise: 3 stars (multistep__eval) *)
+    The proof proceeds by induction on the multi-step reduction
+    sequence that is buried in the hypothesis [normal_form_of t t']. *)
+(** Make sure you understand the statement before you start to
+    work on the proof.  *)
 
+(** **** Exercise: 3 stars (multistep__eval)  *)
 Theorem multistep__eval : forall t t',
   normal_form_of t t' -> exists n, t' = C n /\ t || n.
 Proof.
-  unfold normal_form_of. unfold step_normal_form.
-  intros. destruct H as [H1 H2]. apply nf_same_as_value in H2. inversion H2.
-  exists n. split. reflexivity.
-  multi_cases (induction H1) Case; subst.
-  Case "multi_refl". constructor.
-  Case "multi_step". apply step__eval with y. assumption.
-   apply IHmulti. constructor. reflexivity.
-Qed.
+  (* FILL IN HERE *) Admitted.
+(** [] *)
 
-(* Additional Exercises *)
+(* ########################################################### *)
+(** ** Additional Exercises *)
 
-(* Exercise: 3 stars, optional (interp_tm) *)
+(** **** Exercise: 3 stars, optional (interp_tm)  *)
+(** Remember that we also defined big-step evaluation of [tm]s as a
+    function [evalF].  Prove that it is equivalent to the existing
+    semantics.
+
+    Hint: we just proved that [eval] and [multistep] are
+    equivalent, so logically it doesn't matter which you choose.
+    One will be easier than the other, though!  *)
 
 Theorem evalF_eval : forall t n,
   evalF t = n <-> t || n.
 Proof.
-  split.
-  Case "->". generalize dependent n. tm_cases (induction t) SCase; intros.
-    SCase "C". simpl in H. subst. constructor.
-    SCase "P". simpl in H. subst. apply E_Plus.
-      apply IHt1. reflexivity.
-      apply IHt2. reflexivity.
-  Case "<-". intros.
-    eval_cases (induction H) SCase; subst; reflexivity.
-Qed.
+  (* FILL IN HERE *) Admitted.
+(** [] *)
 
-(* Exercise: 4 stars (combined_properties) *)
-
+(** **** Exercise: 4 stars (combined_properties)  *)
+(** We've considered the arithmetic and conditional expressions
+    separately.  This exercise explores how the two interact. *)
 
 Module Combined.
 
@@ -691,31 +1283,40 @@ Tactic Notation "step_cases" tactic(first) ident(c) :=
   | Case_aux c "ST_Plus1" | Case_aux c "ST_Plus2"
   | Case_aux c "ST_IfTrue" | Case_aux c "ST_IfFalse" | Case_aux c "ST_If" ].
 
-Theorem step_deterministic:
-  deterministic step.
-Proof.
-  unfold deterministic. intros x y1 y2 H1 H2.
-  generalize dependent y2.
-  step_cases (induction H1) Case; intros; inversion H2; subst; try(solve by inversion 2); try(reflexivity).
-  Case "ST_Plus1". apply IHstep in H4. subst. reflexivity.
-  Case "ST_Plus2". apply IHstep in H6. subst. reflexivity.
-  Case "ST_If". apply IHstep in H5. subst. reflexivity.
-Qed.
+(** Earlier, we separately proved for both plus- and if-expressions...
 
-Theorem strong_progress : exists t,
-  ~ (value t \/ (exists t', t ==> t')).
-Proof.
-  unfold not.
-  exists (tif (C 0) (C 0) (C 0)).
-  intros. destruct H as [H1 | H2]; try (solve by inversion 3).
-Qed.
+    - that the step relation was deterministic, and
+
+    - a strong progress lemma, stating that every term is either a
+      value or can take a step.
+
+    Prove or disprove these two properties for the combined language. *)
+
+(* FILL IN HERE *)
+(** [] *)
 
 End Combined.
 
-(* Small-Step Imp *)
+
+(* ########################################################### *)
+(** * Small-Step Imp *)
+
+(** For a more serious example, here is the small-step version of the
+    Imp operational semantics.  *)
+
+(** The small-step evaluation relations for arithmetic and boolean
+    expressions are straightforward extensions of the tiny language
+    we've been working up to now.  To make them easier to read, we
+    introduce the symbolic notations [==>a] and [==>b], respectively,
+    for the arithmetic and boolean step relations. *)
 
 Inductive aval : aexp -> Prop :=
   av_num : forall n, aval (ANum n).
+
+(** We are not actually going to bother to define boolean
+    values, since they aren't needed in the definition of [==>b]
+    below (why?), though they might be if our language were a bit
+    larger (why?). *)
 
 Reserved Notation " t '/' st '==>a' t' " (at level 40, st at level 39).
 
@@ -752,9 +1353,9 @@ Inductive astep : state -> aexp -> aexp -> Prop :=
 
     where " t '/' st '==>a' t' " := (astep st t t').
 
-Reserved Notation " t '/' st '==>b' t' " (at level 40, st at level 39).
+  Reserved Notation " t '/' st '==>b' t' " (at level 40, st at level 39).
 
-Inductive bstep : state -> bexp -> bexp -> Prop :=
+  Inductive bstep : state -> bexp -> bexp -> Prop :=
   | BS_Eq : forall st n1 n2,
       (BEq (ANum n1) (ANum n2)) / st ==>b
       (if (beq_nat n1 n2) then BTrue else BFalse)
@@ -797,6 +1398,28 @@ Inductive bstep : state -> bexp -> bexp -> Prop :=
 
   where " t '/' st '==>b' t' " := (bstep st t t').
 
+(** The semantics of commands is the interesting part.  We need two
+    small tricks to make it work:
+
+       - We use [SKIP] as a "command value" -- i.e., a command that
+         has reached a normal form.
+
+            - An assignment command reduces to [SKIP] (and an updated
+              state).
+
+            - The sequencing command waits until its left-hand
+              subcommand has reduced to [SKIP], then throws it away so
+              that reduction can continue with the right-hand
+              subcommand.
+
+       - We reduce a [WHILE] command by transforming it into a
+         conditional followed by the same [WHILE].  *)
+
+(** (There are other ways of achieving the effect of the latter
+   trick, but they all share the feature that the original [WHILE]
+   command needs to be saved somewhere while a single copy of the loop
+   body is being evaluated.) *)
+
 Reserved Notation " t '/' st '==>' t' '/' st' "
                   (at level 40, st at level 39, t' at level 39).
 
@@ -823,6 +1446,17 @@ Inductive cstep : (com * state) -> (com * state) -> Prop :=
       ==> (IFB b THEN (c1;; (WHILE b DO c1 END)) ELSE SKIP FI) / st
 
   where " t '/' st '==>' t' '/' st' " := (cstep (t,st) (t',st')).
+
+
+(* ########################################################### *)
+(** * Concurrent Imp *)
+
+(** Finally, to show the power of this definitional style, let's
+    enrich Imp with a new form of command that runs two subcommands in
+    parallel and terminates when both have terminated.  To reflect the
+    unpredictability of scheduling, the actions of the subcommands may
+    be interleaved in any order, but they share the same memory and
+    can communicate by reading and writing the same variables. *)
 
 Module CImp.
 
@@ -893,6 +1527,14 @@ Notation " t '/' st '==>*' t' '/' st' " :=
    (multi cstep  (t,st) (t',st'))
    (at level 40, st at level 39, t' at level 39).
 
+
+
+
+
+(** Among the many interesting properties of this language is the fact
+    that the following program can terminate with the variable [X] set
+    to any value... *)
+
 Definition par_loop : com :=
   PAR
     Y ::= ANum 1
@@ -901,6 +1543,8 @@ Definition par_loop : com :=
       X ::= APlus (AId X) (ANum 1)
     END
   END.
+
+(** In particular, it can terminate with [X] set to [0]: *)
 
 Example par_loop_example_0:
   exists st',
@@ -920,6 +1564,8 @@ Proof.
   eapply multi_step. apply CS_ParDone.
   eapply multi_refl.
   reflexivity. Qed.
+
+(** It can also terminate with [X] set to [2]: *)
 
 Example par_loop_example_2:
   exists st',
@@ -966,44 +1612,27 @@ Proof.
   eapply multi_refl.
   reflexivity. Qed.
 
-Require Coq.omega.Omega.
-Ltac omega := Coq.omega.Omega.omega.
+(** More generally... *)
 
 (** **** Exercise: 3 stars, optional  *)
 Lemma par_body_n__Sn : forall n st,
   st X = n /\ st Y = 0 ->
   par_loop / st ==>* par_loop / (update st X (S n)).
 Proof.
-  intros. unfold par_loop. destruct H as [H1 H2].
-  eapply multi_step. apply CS_Par2. apply CS_While.
-  eapply multi_step. apply CS_Par2. apply CS_IfStep. apply BS_Eq1. apply AS_Id.
-  eapply multi_step. apply CS_Par2. apply CS_IfStep. rewrite H2. apply BS_Eq.
-  eapply multi_step. apply CS_Par2. simpl. apply CS_IfTrue.
-  eapply multi_step. apply CS_Par2. apply CS_SeqStep. apply CS_AssStep. apply AS_Plus1. apply AS_Id. rewrite H1.
-  eapply multi_step. apply CS_Par2. apply CS_SeqStep. apply CS_AssStep. apply AS_Plus.
-  eapply multi_step. apply CS_Par2. apply CS_SeqStep. apply CS_Ass.
-  eapply multi_step. apply CS_Par2. apply CS_SeqFinish.
-  assert (n + 1 = S n). omega. rewrite H.
-  eapply multi_refl.
-Qed.
+  (* FILL IN HERE *) Admitted.
+(** [] *)
 
-(* Exercise: 3 stars, optional *)
-
+(** **** Exercise: 3 stars, optional  *)
 Lemma par_body_n : forall n st,
   st X = 0 /\ st Y = 0 ->
   exists st',
     par_loop / st ==>*  par_loop / st' /\ st' X = n /\ st' Y = 0.
 Proof.
-  intros. unfold par_loop.
-  induction n as [| n'].
-  exists st. split. apply multi_refl. assumption.
-  inversion IHn'. clear IHn'.
-  destruct H0 as [ H1 [H2 H3]].
-  exists (update x X (S n')). split.
-  eapply multi_trans. apply H1.
-  apply par_body_n__Sn. split; assumption.
-  split. reflexivity. unfold update. simpl. assumption.
-Qed.
+  (* FILL IN HERE *) Admitted.
+(** [] *)
+
+(** ... the above loop can exit with [X] having any value
+    whatsoever. *)
 
 Theorem par_loop_any_X:
   forall n, exists st',
@@ -1032,3 +1661,50 @@ Proof.
 Qed.
 
 End CImp.
+
+(* ########################################################### *)
+(** * A Small-Step Stack Machine *)
+
+(** Last example: a small-step semantics for the stack machine example
+    from Imp.v. *)
+
+Definition stack := list nat.
+Definition prog  := list sinstr.
+
+Inductive stack_step : state -> prog * stack -> prog * stack -> Prop :=
+  | SS_Push : forall st stk n p',
+    stack_step st (SPush n :: p', stk)      (p', n :: stk)
+  | SS_Load : forall st stk i p',
+    stack_step st (SLoad i :: p', stk)      (p', st i :: stk)
+  | SS_Plus : forall st stk n m p',
+    stack_step st (SPlus :: p', n::m::stk)  (p', (m+n)::stk)
+  | SS_Minus : forall st stk n m p',
+    stack_step st (SMinus :: p', n::m::stk) (p', (m-n)::stk)
+  | SS_Mult : forall st stk n m p',
+    stack_step st (SMult :: p', n::m::stk)  (p', (m*n)::stk).
+
+Theorem stack_step_deterministic : forall st,
+  deterministic (stack_step st).
+Proof.
+  unfold deterministic. intros st x y1 y2 H1 H2.
+  induction H1; inversion H2; reflexivity.
+Qed.
+
+Definition stack_multistep st := multi (stack_step st).
+
+(** **** Exercise: 3 stars, advanced (compiler_is_correct)  *)
+(** Remember the definition of [compile] for [aexp] given in the
+    [Imp] chapter. We want now to prove [compile] correct with respect
+    to the stack machine.
+
+    State what it means for the compiler to be correct according to
+    the stack machine small step semantics and then prove it. *)
+
+Definition compiler_is_correct_statement : Prop :=
+(* FILL IN HERE *) admit.
+
+
+Theorem compiler_is_correct : compiler_is_correct_statement.
+Proof.
+(* FILL IN HERE *) Admitted.
+(** [] *)
